examples/scache/Cache.i.dfy
@@ -192,10 +192,10 @@ module CacheImpl {
     {
       var cache_idx := ci * (CHUNK_SIZE as uint32) + i;   
 
-      linear var write_back_r;
+      linear var write_back_r, ticket;
       /*readonly*/ linear var readonly_handle_maybe: maybe<RWLock.Handle>;
       var do_write_back;
-      do_write_back, write_back_r, readonly_handle_maybe :=
+      do_write_back, write_back_r, readonly_handle_maybe, ticket :=
           try_acquire_writeback(
               c.status[cache_idx],
               c.key(cache_idx as int),
@@ -207,20 +207,25 @@ module CacheImpl {
             cache_entry, data, idx) := readonly_handle;
 
         var disk_idx := ptr_read(c.disk_idx_of_entry[cache_idx], idx);
-        if disk_idx != -1 {
-          linear var wgs := DiskIO.WritebackGhostState(
-              unwrap(write_back_r), cache_entry, idx);
+        assert disk_idx != -1;
 
-          DiskIO.disk_writeback_async(disk_idx as uint64, c.data[cache_idx],
-              data, wgs);
-        } else {
+        linear var wgs := DiskIO.WritebackGhostState(
+            unwrap(write_back_r), cache_entry, idx);
+
+        DiskIO.disk_writeback_async(
+            disk_idx as uint64,
+            c.data[cache_idx],
+            data, wgs, unwrap(ticket));
+
+        /*} else {
           readonly_handle := RWLock.CacheEntryHandle(cache_entry, data, idx);
           release_writeback(c.status[cache_idx], c.key(cache_idx as int),
               unwrap(write_back_r), readonly_handle);
-        }
+        }*/
       } else {
         var _ := discard(readonly_handle_maybe);
         var _ := discard(write_back_r);
+        var _ := discard(ticket);
       }
 
       i := i + 1;
